src/program_proof/rsm/distx/program/txn.v
@@ -18,13 +18,68 @@ Section program.
   Definition own_txn (txn : loc) (tid : nat) (γ : distx_names) (τ : gname) : iProp Σ.
   Admitted.
 
+  Definition own_txn_ready_ptgs (txn : loc) (tid : nat) (γ : distx_names) (τ : gname) : iProp Σ.
+  Admitted.
+
+  Theorem wp_KeyToGroup (key : string) :
+    {{{ True }}}
+      KeyToGroup #(LitString key)
+    {{{ (gid : u64), RET #gid; ⌜key_to_group key = (uint.nat gid)⌝ }}}.
+  Proof.
+    (*@ func KeyToGroup(key string) uint64 {                                    @*)
+    (*@     // TODO                                                             @*)
+    (*@     return 0                                                            @*)
+    (*@ }                                                                       @*)
+  Admitted.
+
+  Theorem wp_Txn__Read (txn : loc) (tid : nat) (key : string) (value : dbval) γ τ :
+    {{{ own_txn txn tid γ τ ∗ txn_ptsto τ key value }}}
+      Txn__Read #txn #(LitString key)
+    {{{ RET (dbval_to_val value); own_txn txn tid γ τ ∗ txn_ptsto τ key value }}}.
+  Proof.
+    (*@ func (txn *Txn) Read(key string) Value {                                @*)
+    (*@     gid := KeyToGroup(key)                                              @*)
+    (*@                                                                         @*)
+    (*@     pwrs := txn.wrs[gid]                                                @*)
+    (*@     vlocal, ok := pwrs[key]                                             @*)
+    (*@     if ok {                                                             @*)
+    (*@         return vlocal                                                   @*)
+    (*@     }                                                                   @*)
+    (*@                                                                         @*)
+    (*@     rg := txn.rgs[gid]                                                  @*)
+    (*@     v := rg.Read(txn.ts, key)                                           @*)
+    (*@     return v                                                            @*)
+    (*@ }                                                                       @*)
+  Admitted.
+
+  Theorem wp_Txn__Write (txn : loc) (tid : nat) (key : string) (value : string) γ τ :
+    {{{ own_txn txn tid γ τ ∗ (∃ vprev, txn_ptsto τ key vprev) }}}
+      Txn__Write #txn #(LitString key) #(LitString value)
+    {{{ RET #(); own_txn txn tid γ τ ∗ txn_ptsto τ key (Some value) }}}.
+  Proof.
+    (*@ func (txn *Txn) Write(key string, value string) {                       @*)
+    (*@     gid := KeyToGroup(key)                                              @*)
+    (*@     pwrs := txn.wrs[gid]                                                @*)
+    (*@     v := Value{                                                         @*)
+    (*@         b : true,                                                       @*)
+    (*@         s : value,                                                      @*)
+    (*@     }                                                                   @*)
+    (*@     pwrs[key] = v                                                       @*)
+    (*@ }                                                                       @*)
+  Admitted.
+
   Theorem wp_Txn__Delete (txn : loc) (tid : nat) (key : string) (value : dbval) γ τ :
     {{{ own_txn txn tid γ τ ∗ txn_ptsto τ key value }}}
       Txn__Delete #txn #(LitString key)
     {{{ RET #(); own_txn txn tid γ τ ∗ txn_ptsto τ key None }}}.
   Proof.
     (*@ func (txn *Txn) Delete(key string) {                                    @*)
-    (*@     // TODO                                                             @*)
+    (*@     gid := KeyToGroup(key)                                              @*)
+    (*@     pwrs := txn.wrs[gid]                                                @*)
+    (*@     v := Value{                                                         @*)
+    (*@         b : false,                                                      @*)
+    (*@     }                                                                   @*)
+    (*@     pwrs[key] = v                                                       @*)
     (*@ }                                                                       @*)
   Admitted.
 
@@ -35,25 +90,31 @@ Section program.
     {{{ RET #(); own_txn_uninit txn γ }}}.
   Proof.
     (*@ func (txn *Txn) abort() {                                               @*)
-    (*@     for _, rg := range(txn.rgs) {                                       @*)
+    (*@     for _, gid := range(txn.ptgs) {                                     @*)
+    (*@         rg := txn.rgs[gid]                                              @*)
+    (*@         pwrs := txn.wrs[gid]                                            @*)
+    (*@                                                                         @*)
     (*@         // Should abort in parallel.                                    @*)
-    (*@         if uint64(len(rg.wrs)) != 0 {                                   @*)
+    (*@         if uint64(len(pwrs)) != 0 {                                     @*)
     (*@             rg.Abort(txn.ts)                                            @*)
     (*@         }                                                               @*)
     (*@     }                                                                   @*)
     (*@ }                                                                       @*)
   Admitted.
 
-  Theorem wp_Txn__commit (txn : loc) (tid : nat) (wrs : dbmap) (γ : distx_names) (τ : gname) :
+  Theorem wp_Txn__commit (txn : loc) (tid : nat) (wrs : dbmap) γ τ :
     txnres_cmt γ tid wrs -∗
     {{{ own_txn txn tid γ τ }}}
       Txn__commit #txn
     {{{ RET #(); own_txn_uninit txn γ }}}.
   Proof.
     (*@ func (txn *Txn) commit() {                                              @*)
-    (*@     for _, rg := range(txn.rgs) {                                       @*)
+    (*@     for _, gid := range(txn.ptgs) {                                     @*)
+    (*@         rg := txn.rgs[gid]                                              @*)
+    (*@         pwrs := txn.wrs[gid]                                            @*)
+    (*@                                                                         @*)
     (*@         // Should commit in parallel.                                   @*)
-    (*@         if uint64(len(rg.wrs)) != 0 {                                   @*)
+    (*@         if uint64(len(pwrs)) != 0 {                                     @*)
     (*@             rg.Commit(txn.ts)                                           @*)
     (*@         }                                                               @*)
     (*@     }                                                                   @*)
@@ -74,37 +135,54 @@ Section program.
     (*@ }                                                                       @*)
   Admitted.
 
+  Theorem wp_Txn__setptgs txn tid γ τ :
+    {{{ own_txn txn tid γ τ }}}
+      Txn__setptgs #txn
+    {{{ RET #(); own_txn_ready_ptgs txn tid γ τ }}}.
+  Proof.
+    (*@ func (txn *Txn) setptgs() {                                             @*)
+    (*@     var ptgs []uint64 = make([]uint64, 0)                               @*)
+    (*@                                                                         @*)
+    (*@     for gid, pwrs := range(txn.wrs) {                                   @*)
+    (*@         if uint64(len(pwrs)) != 0 {                                     @*)
+    (*@             ptgs = append(ptgs, gid)                                    @*)
+    (*@         }                                                               @*)
+    (*@     }                                                                   @*)
+    (*@     txn.ptgs = ptgs                                                     @*)
+    (*@ }                                                                       @*)
+  Admitted.
+
   Definition groups_txnst γ (ts : nat) (st : txnst) : iProp Σ :=
     match st with
     | StPrepared wrs => all_prepared γ ts wrs
-    | StCommitted => True
-    | StAborted => some_aborted γ ts
+    | StCommitted => (∃ wrs, txnres_cmt γ ts wrs)
+    | StAborted => txnres_abt γ ts
     end.
 
-  Theorem wp_Txn__prepare (txn : loc) (tid : nat) (γ : distx_names) (τ : gname) :
+  Theorem wp_Txn__prepare txn tid γ τ :
     {{{ own_txn txn tid γ τ }}}
       Txn__prepare #txn
     {{{ (status : txnst), RET #(txnst_to_u64 status);
-        own_txn txn tid γ τ ∗ groups_txnst γ tid status
+        own_txn_ready_ptgs txn tid γ τ ∗ groups_txnst γ tid status
     }}}.
   Proof.
     (*@ func (txn *Txn) prepare() uint64 {                                      @*)
     (*@     var status = TXN_PREPARED                                           @*)
-    (*@     var gid uint64 = 0                                                  @*)
     (*@                                                                         @*)
-    (*@     for gid < uint64(len(txn.rgs)) {                                    @*)
+    (*@     txn.setptgs()                                                       @*)
+    (*@                                                                         @*)
+    (*@     var i uint64 = 0                                                    @*)
+    (*@     for i < uint64(len(txn.ptgs)) {                                     @*)
+    (*@         gid := txn.ptgs[i]                                              @*)
     (*@         rg := txn.rgs[gid]                                              @*)
+    (*@         pwrs := txn.wrs[gid]                                            @*)
     (*@                                                                         @*)
-    (*@         if uint64(len(rg.wrs)) == 0 {                                   @*)
-    (*@             continue                                                    @*)
-    (*@         }                                                               @*)
-    (*@                                                                         @*)
-    (*@         status = rg.Prepare(txn.ts)                                     @*)
+    (*@         status = rg.Prepare(txn.ts, slicem(pwrs))                       @*)
     (*@         if status != TXN_PREPARED {                                     @*)
     (*@             break                                                       @*)
     (*@         }                                                               @*)
     (*@                                                                         @*)
-    (*@         gid++                                                           @*)
+    (*@         i++                                                             @*)
     (*@     }                                                                   @*)
     (*@                                                                         @*)
     (*@     return status                                                       @*)
@@ -121,7 +199,7 @@ Section program.
     (∀ ok : bool,
        (own_txn txn tid γ τ ∗
         if ok
-        then ∃ w, ⌜Q r w ∧ dom r = dom w⌝ ∗ (Rc r w ∧ Ra r) ∗ txn_ptstos τ w
+        then ∃ w, ⌜Q r w ∧ dom w ⊆ dom r⌝ ∗ (Rc r w ∧ Ra r) ∗ txn_ptstos τ w
         else Ra r) -∗ Φ #ok) -∗
     WP body #txn {{ v, Φ v }}.
 
@@ -133,7 +211,7 @@ Section program.
     ⊢ {{{ own_txn_uninit txn γ ∗ (∀ tid r τ, spec_body body txn tid r P Q Rc Ra γ τ) }}}
       <<< ∀∀ (r : dbmap), ⌜P r⌝ ∗ db_ptstos γ r >>>
         Txn__Run #txn body @ ↑distxN
-      <<< ∃∃ (ok : bool) (w : dbmap), if ok then ⌜Q r w⌝ ∗ db_ptstos γ w else db_ptstos γ r >>>
+      <<< ∃∃ (ok : bool) (w : dbmap), if ok then ⌜Q r w⌝ ∗ db_ptstos γ (w ∪ r) else db_ptstos γ r >>>
       {{{ RET #ok; own_txn_uninit txn γ ∗ if ok then Rc r w else Ra r }}}.
   Proof.
     (*@ func (txn *Txn) Run(body func(txn *Txn) bool) bool {                    @*)
