src/program_proof/rsm/distx/program/replica_group.v
@@ -1,11 +1,21 @@
 From Perennial.program_proof.rsm.distx Require Import prelude.
-From Perennial.program_proof.rsm.distx.program Require Import replica.
+From Perennial.program_proof.rsm.distx.program Require Import replica txnlog.
 From Goose.github_com.mit_pdos.rsm Require Import distx.
 
 Section program.
   Context `{!heapGS Σ, !distx_ghostG Σ}.
 
   Definition is_rg (rg : loc) (gid : groupid) (γ : distx_names) : iProp Σ.
+  Admitted.
+
+  Theorem wp_ReplicaGroup__changeLeader (rg : loc) :
+    {{{ True }}}
+      ReplicaGroup__changeLeader #rg
+    {{{ RET #(); True }}}.
+  Proof.
+    (*@ func (rg *ReplicaGroup) changeLeader() {                                @*)
+    (*@     // TODO                                                             @*)
+    (*@ }                                                                       @*)
   Admitted.
 
   Theorem wp_ReplicaGroup__Abort (rg : loc) (ts : u64) (gid : groupid) γ :
@@ -48,19 +58,42 @@ Section program.
     (*@ }                                                                       @*)
   Admitted.
 
-  Theorem wp_ReplicaGroup__Prepare (rg : loc) (ts : u64) (gid : groupid) γ :
-    is_rg rg gid γ -∗
+  Theorem wp_ReplicaGroup__Read (rg : loc) (ts : u64) (key : string) :
     {{{ True }}}
-      ReplicaGroup__Prepare #rg #ts
+      ReplicaGroup__Read #rg #ts #(LitString key)
+    {{{ (value : dbval), RET (dbval_to_val value); True }}}.
+  Proof.
+    (*@ func (rg *ReplicaGroup) Read(ts uint64, key string) Value {             @*)
+    (*@     var value Value                                                     @*)
+    (*@                                                                         @*)
+    (*@     // Find the right replica to prepare; retry until success.          @*)
+    (*@     for {                                                               @*)
+    (*@         rp := rg.rps[rg.leader]                                         @*)
+    (*@         v, ok := rp.Read(ts, key)                                       @*)
+    (*@         if ok {                                                         @*)
+    (*@             value = v                                                   @*)
+    (*@             break                                                       @*)
+    (*@         }                                                               @*)
+    (*@         rg.changeLeader()                                               @*)
+    (*@     }                                                                   @*)
+    (*@                                                                         @*)
+    (*@     return value                                                        @*)
+    (*@ }                                                                       @*)
+  Admitted.
+
+  Theorem wp_ReplicaGroup__Prepare
+    (rg : loc) (ts : u64) (pwrsS : Slice.t) (pwrsL : list dbmod) (pwrs : dbmap) gid γ :
+    {{{ own_dbmap_in_slice pwrsS pwrsL pwrs }}}
+      ReplicaGroup__Prepare #rg #ts (to_val pwrsS)
     {{{ (st : txnst), RET #(txnst_to_u64 st); txn_token γ gid (uint.nat ts) st }}}.
   Proof.
-    (*@ func (rg *ReplicaGroup) Prepare(ts uint64) uint64 {                     @*)
+    (*@ func (rg *ReplicaGroup) Prepare(ts uint64, pwrs []WriteEntry) uint64 {  @*)
     (*@     var status uint64                                                   @*)
     (*@                                                                         @*)
     (*@     // Find the right replica to prepare; retry until success.          @*)
     (*@     for {                                                               @*)
     (*@         rp := rg.rps[rg.leader]                                         @*)
-    (*@         s, ok := rp.Prepare(ts, slicem(rg.wrs))                         @*)
+    (*@         s, ok := rp.Prepare(ts, pwrs)                                   @*)
     (*@         if ok {                                                         @*)
     (*@             status = s                                                  @*)
     (*@             break                                                       @*)
